Progress on top-level memory safety for AES128-GCM

code/experimental/aes-gcm/Hacl.AES_128_GCM.M32.fst
@@ -11,7 +11,7 @@ open Hacl.Gf128.PreComp
 module ST = FStar.HyperStack.ST
 
 
-#set-options "--z3rlimit 10"
+#set-options "--z3rlimit 500"
 
 let aes_gcm_ctx_len = 396ul
 
@@ -24,7 +24,7 @@ val aes128_gcm_init:
   -> nonce: lbuffer uint8 12ul ->
   Stack unit
   (requires (fun h -> live h ctx /\ live h key /\ live h nonce))
-  (ensures (fun h0 _ h1 -> modifies (loc ctx) h0 h1))
+  (ensures (fun h0 _ h1 -> modifies1 ctx h0 h1))
 
 let aes128_gcm_init ctx key nonce =
   push_frame();
@@ -40,8 +40,7 @@ let aes128_gcm_init ctx key nonce =
   gcm_init gcm_ctx gcm_key;
   ctx.(394ul) <- uint_from_bytes_le #U64 (sub tag_mix 0ul 8ul);
   ctx.(395ul) <- uint_from_bytes_le #U64 (sub tag_mix 8ul 8ul);
-  pop_frame();
-  admit()
+  pop_frame()
 
 
 val aes128_gcm_encrypt:
@@ -52,11 +51,17 @@ val aes128_gcm_encrypt:
   -> aad_len: size_t
   -> aad: lbuffer uint8 aad_len ->
   Stack unit
-  (requires (fun h -> live h out /\ live h text /\ live h aad /\ live h ctx))
-  (ensures (fun h0 _ h1 -> modifies (loc out) h0 h1))
+  (requires (fun h -> live h out /\ live h text /\ live h aad /\ live h ctx
+                 /\ disjoint out ctx
+                 /\ disjoint ctx text
+                 /\ disjoint ctx aad
+                 /\ disjoint out text
+                 /\ disjoint out aad))
+  (ensures (fun h0 _ h1 -> modifies2 out ctx h0 h1))
 
 let aes128_gcm_encrypt ctx len out text aad_len aad =
   push_frame();
+  let tmp = create 16ul (u8 0) in
   let cip = sub out (size 0) len in
   let aes_ctx = sub ctx (size 0) (size 128) in
   let gcm_ctx = sub ctx (size 128) (size 266) in
@@ -64,7 +69,6 @@ let aes128_gcm_encrypt ctx len out text aad_len aad =
   aes128_ctr len cip text aes_ctx (size 2);
   gcm_update_blocks_padded gcm_ctx aad_len aad;
   gcm_update_blocks_padded gcm_ctx len cip;
-  let tmp = create 16ul (u8 0) in
   uint_to_bytes_be #U64 (sub tmp (size 0) (size 8)) (to_u64 (aad_len *. 8ul));
   uint_to_bytes_be #U64 (sub tmp (size 8) (size 8)) (to_u64 (len *. 8ul));
   gcm_update_blocks gcm_ctx (size 16) tmp;
@@ -75,45 +79,53 @@ let aes128_gcm_encrypt ctx len out text aad_len aad =
   let tmp1 = tmp1 ^. tag_mix.(1ul) in
   uint_to_bytes_le #U64 (sub out len 8ul) tmp0;
   uint_to_bytes_le #U64 (sub out (len +. 8ul) 8ul) tmp1;
-  pop_frame();
-  admit()
+  pop_frame()
 
 
 val aes128_gcm_decrypt:
     ctx: aes_gcm_ctx
-  -> len: size_t
+  -> len: size_t{v len + 16 <= max_size_t}
   -> out: lbuffer uint8 len
   -> cipher: lbuffer uint8 (len +. 16ul)
   -> aad_len: size_t
   -> aad: lbuffer uint8 aad_len ->
   Stack bool
-  (requires (fun h -> live h out /\ live h cipher /\ live h aad /\ live h ctx))
-  (ensures (fun h0 r h1 -> modifies (loc out) h0 h1))
+  (requires (fun h -> live h out /\ live h cipher /\ live h aad /\ live h ctx
+                 /\ disjoint out ctx
+                 /\ disjoint ctx cipher
+                 /\ disjoint ctx aad
+                 /\ disjoint out cipher
+                 /\ disjoint out aad))
+  (ensures (fun h0 r h1 -> modifies1 out h0 h1))
+
+#reset-options "--z3rlimit 500 --max_fuel 1"
 
 let aes128_gcm_decrypt ctx len out cipher aad_len aad =
   push_frame();
+  let scratch = create 16ul (u8 0) in
+  let ciphertext = sub cipher 0ul len in
   let aes_ctx = sub ctx (size 0) (size 128) in
   let gcm_ctx = sub ctx (size 128) (size 266) in
   let tag_mix = sub ctx (size 394) (size 2) in
   gcm_update_blocks_padded gcm_ctx aad_len aad;
-  gcm_update_blocks_padded gcm_ctx len cipher;
-  let tmp = create 16ul (u8 0) in
-  uint_to_bytes_be #U64 (sub tmp (size 0) (size 8)) (to_u64 (aad_len *. size 8));
-  uint_to_bytes_be #U64 (sub tmp (size 8) (size 8)) (to_u64 (len *. size 8));
-  gcm_update_blocks gcm_ctx (size 16) tmp;
-  gcm_emit tmp gcm_ctx;
-  let tmp0 = uint_from_bytes_le #U64 (sub tmp 0ul 8ul) in
-  let tmp1 = uint_from_bytes_le #U64 (sub tmp 8ul 8ul) in
-  let tmp0 = tmp0 ^. tag_mix.(0ul) in
-  let tmp1 = tmp1 ^. tag_mix.(1ul) in
-  uint_to_bytes_le #U64 (sub tmp 0ul 8ul) tmp0;
-  uint_to_bytes_le #U64 (sub tmp 8ul 8ul) tmp1;
+  gcm_update_blocks_padded gcm_ctx len ciphertext;
+  uint_to_bytes_be #U64 (sub scratch (size 0) (size 8)) (to_u64 (aad_len *. size 8));
+  uint_to_bytes_be #U64 (sub scratch (size 8) (size 8)) (to_u64 (len *. size 8));
+  gcm_update_blocks gcm_ctx (size 16) scratch;
+  gcm_emit scratch gcm_ctx;
+  let scratch0 = uint_from_bytes_le #U64 (sub scratch 0ul 8ul) in
+  let scratch1 = uint_from_bytes_le #U64 (sub scratch 8ul 8ul) in
+  let scratch0 = scratch0 ^. tag_mix.(0ul) in
+  let scratch1 = scratch1 ^. tag_mix.(1ul) in
+  uint_to_bytes_le #U64 (sub scratch 0ul 8ul) scratch0;
+  uint_to_bytes_le #U64 (sub scratch 8ul 8ul) scratch1;
   let tag = sub cipher len (size 16) in
   let res = create 1ul (u8 0) in
   let h1 = ST.get() in
   loop_nospec #h1 (size 16) res
-    (fun i -> res.(0ul) <- res.(0ul) |. (tmp.(i) ^. tag.(i)));
+    (fun i -> res.(0ul) <- res.(0ul) |. (scratch.(i) ^. tag.(i)));
   let r = res.(size 0) in
+  admit();
   if Lib.RawIntTypes.u8_to_UInt8 r = 0uy then (
     let cip = sub cipher (size 0) len in
     aes128_ctr len out cip aes_ctx (size 2);
