code/experimental/aes-gcm/Hacl.AES_128_GCM.NI.fst
@@ -24,7 +24,7 @@ val aes128_gcm_init:
   -> nonce: lbuffer uint8 12ul ->
   Stack unit
   (requires (fun h -> live h ctx /\ live h key /\ live h nonce))
-  (ensures (fun h0 _ h1 -> modifies (loc ctx) h0 h1))
+  (ensures (fun h0 _ h1 -> modifies1 ctx h0 h1))
 
 let aes128_gcm_init ctx key nonce =
   push_frame();
@@ -39,9 +39,9 @@ let aes128_gcm_init ctx key nonce =
   aes128_key_block tag_mix aes_ctx (size 1);
   gcm_init gcm_ctx gcm_key;
   ctx.(21ul) <- vec128_load_le tag_mix;
-  pop_frame();
-  admit()
+  pop_frame()
 
+#reset-options "--z3rlimit 500 --max_fuel 1"
 
 val aes128_gcm_encrypt:
     ctx: aes_gcm_ctx
@@ -51,8 +51,13 @@ val aes128_gcm_encrypt:
   -> aad_len: size_t
   -> aad: lbuffer uint8 aad_len ->
   Stack unit
-  (requires (fun h -> live h out /\ live h text /\ live h aad /\ live h ctx))
-  (ensures (fun h0 _ h1 -> modifies (loc out) h0 h1))
+  (requires (fun h -> live h out /\ live h text /\ live h aad /\ live h ctx
+                 /\ disjoint out ctx
+                 /\ disjoint out text
+                 /\ disjoint out aad
+                 /\ disjoint ctx text
+                 /\ disjoint ctx aad))
+  (ensures (fun h0 _ h1 -> modifies2 out ctx h0 h1))
 
 let aes128_gcm_encrypt ctx len out text aad_len aad =
   push_frame();
@@ -71,28 +76,33 @@ let aes128_gcm_encrypt ctx len out text aad_len aad =
   let tmp_vec = vec128_load_le tmp in
   let tmp_vec = vec128_xor tmp_vec tag_mix in
   vec128_store_le (sub out len (size 16)) tmp_vec;
-  pop_frame();
-  admit()
+  pop_frame()
 
 
 val aes128_gcm_decrypt:
     ctx: aes_gcm_ctx
-  -> len: size_t
+  -> len: size_t{v len + 16 <= max_size_t}
   -> out: lbuffer uint8 len
   -> cipher: lbuffer uint8 (len +. 16ul)
   -> aad_len: size_t
   -> aad: lbuffer uint8 aad_len ->
   Stack bool
-  (requires (fun h -> live h out /\ live h cipher /\ live h aad /\ live h ctx))
-  (ensures (fun h0 r h1 -> modifies (loc out) h0 h1))
+  (requires (fun h -> live h out /\ live h cipher /\ live h aad /\ live h ctx
+                 /\ disjoint out ctx
+                 /\ disjoint out cipher
+                 /\ disjoint out aad
+                 /\ disjoint ctx cipher
+                 /\ disjoint ctx aad))
+  (ensures (fun h0 r h1 -> modifies2 out ctx h0 h1))
 
 let aes128_gcm_decrypt ctx len out cipher aad_len aad =
   push_frame();
+  let ciphertext = sub cipher 0ul len in
   let aes_ctx = sub ctx (size 0) (size 16) in
   let gcm_ctx = sub ctx (size 16) (size 5) in
   let tag_mix = ctx.(21ul) in
   gcm_update_padded gcm_ctx aad_len aad;
-  gcm_update_padded gcm_ctx len cipher;
+  gcm_update_padded gcm_ctx len ciphertext;
   let tmp = create 16ul (u8 0) in
   uint_to_bytes_be #U64 (sub tmp (size 0) (size 8)) (to_u64 (aad_len *. size 8));
   uint_to_bytes_be #U64 (sub tmp (size 8) (size 8)) (to_u64 (len *. size 8));
@@ -104,6 +114,7 @@ let aes128_gcm_decrypt ctx len out cipher aad_len aad =
   let tag = sub cipher len (size 16) in
   let res = create 1ul (u8 0) in
   let h1 = ST.get() in
+  admit();
   loop_nospec #h1 (size 16) res
     (fun i -> res.(0ul) <- res.(0ul) |. (tmp.(i) ^. tag.(i)));
   let r = res.(size 0) in
